<?xml version="1.0" encoding="UTF-8"?>
<exercises permid="sec_sequences-conc" xmlns:xi="http://www.w3.org/2001/XInclude" xml:id="sec_sequences-conc">
  <title>Chapter Review</title>
  <exercise permid="sec_sequences-conc-e_xo">
    <statement>
      <p permid="sec_sequences-conc-e_xo-p1">
        Find <m>3 + 7 + 11+ \cdots + 427</m>.
      </p>
    </statement>
    <solution permid="sec_sequences-conc-e_xo-s1">
      <p permid="sec_sequences-conc-e_xo-s1-p1">
        <m>\frac{430\cdot 107}{2} = 23005</m>.
      </p>
    </solution>
  </exercise>

  <exercise permid="sec_sequences-conc-e_ag">
    <statement>
      <p permid="sec_sequences-conc-e_ag-p1">
        Consider the sequence <m>2, 6, 10, 14, \ldots, 4n + 6</m>.
      </p>

      <p permid="sec_sequences-conc-e_ag-p2">
        <ol permid="sec_sequences-conc-e_ag-ol1">
          <li permid="sec_sequences-conc-e_ag-ol1-l_j">
            <p permid="sec_sequences-conc-e_ag-ol1-l_j-p1">
              How many terms are there in the sequence?
            </p>
          </li>

          <li permid="sec_sequences-conc-e_ag-ol1-l_s">
            <p permid="sec_sequences-conc-e_ag-ol1-l_s-p1">
              What is the second-to-last term?
            </p>
          </li>

          <li permid="sec_sequences-conc-e_ag-ol1-l_b">
            <p permid="sec_sequences-conc-e_ag-ol1-l_b-p1">
              Find the sum of all the terms in the sequence.
            </p>
          </li>
        </ol>
      </p>
    </statement>
    <solution permid="sec_sequences-conc-e_ag-s1">
      <p permid="sec_sequences-conc-e_ag-s1-p1">
        <ol permid="sec_sequences-conc-e_ag-s1-ol1">
          <li permid="sec_sequences-conc-e_ag-s1-ol1-l_j"><m>n+2</m> terms.</li>

          <li permid="sec_sequences-conc-e_ag-s1-ol1-l_s"><m>4n+2</m>.</li>

          <li permid="sec_sequences-conc-e_ag-s1-ol1-l_b"><m>\frac{(4n+8)(n+2)}{2}</m>.</li>
        </ol>
      </p>
    </solution>
  </exercise>

  <exercise permid="sec_sequences-conc-e_dp">
    <statement>
      <p permid="sec_sequences-conc-e_dp-p1">
        Consider the sequence given by <m>a_n = 2\cdot 5^{n-1}</m>.
      </p>

      <p permid="sec_sequences-conc-e_dp-p2">
        <ol permid="sec_sequences-conc-e_dp-ol1">
          <li permid="sec_sequences-conc-e_dp-ol1-l_j">
            <p permid="sec_sequences-conc-e_dp-ol1-l_j-p1">
              Find the first 4 terms of the sequence.
              What sort of sequence is this?
            </p>
          </li>

          <li permid="sec_sequences-conc-e_dp-ol1-l_s">
            <p permid="sec_sequences-conc-e_dp-ol1-l_s-p1">
              Find the <em>sum</em> of the first 25 terms.
              That is, compute <m>\d\sum_{k=1}^{25}a_k</m>.
            </p>
          </li>
        </ol>
      </p>
    </statement>
    <solution permid="sec_sequences-conc-e_dp-s1">
      <p permid="sec_sequences-conc-e_dp-s1-p1">
        <ol permid="sec_sequences-conc-e_dp-s1-ol1">
          <li permid="sec_sequences-conc-e_dp-s1-ol1-l_j">
            <m>2, 10, 50, 250, \ldots</m> The sequence is geometric.
          </li>

          <li permid="sec_sequences-conc-e_dp-s1-ol1-l_s"><m>\frac{2 - 2\cdot 5^{25}}{-4}</m>.</li>
        </ol>
      </p>
    </solution>
  </exercise>

  <exercise permid="sec_sequences-conc-e_gy">
    <statement>
      <p permid="sec_sequences-conc-e_gy-p1">
        Consider the sequence <m>5, 11, 19, 29, 41, 55,\ldots</m>.
        Assume <m>a_1 = 5</m>.
      </p>

      <p permid="sec_sequences-conc-e_gy-p2">
        <ol permid="sec_sequences-conc-e_gy-ol1">
          <li permid="sec_sequences-conc-e_gy-ol1-l_j">
            <p permid="sec_sequences-conc-e_gy-ol1-l_j-p1">
              Find a closed formula for <m>a_n</m>,
              the <m>n</m>th term of the sequence,
              by writing each term as a sum of a sequence.
              Hint: first find <m>a_0</m>, but ignore it when collapsing the sum.
            </p>
          </li>

          <li permid="sec_sequences-conc-e_gy-ol1-l_s">
            <p permid="sec_sequences-conc-e_gy-ol1-l_s-p1">
              Find a closed formula again,
              this time using either polynomial fitting or the characteristic root technique
              (whichever is appropriate).
              Show your work.
            </p>
          </li>

          <li permid="sec_sequences-conc-e_gy-ol1-l_b">
            <p permid="sec_sequences-conc-e_gy-ol1-l_b-p1">
              Find a closed formula once again,
              this time by recognizing the sequence as a modification to some well known sequence(s).
              Explain.
            </p>
          </li>
        </ol>
      </p>
    </statement>
  </exercise>

  <exercise permid="sec_sequences-conc-e_jq">
    <statement>
      <p permid="sec_sequences-conc-e_jq-p1">
        Use polynomial fitting to find a closed formula for the sequence <m>(a_n)_{n\ge 1}</m>:
        <me permid="sec_sequences-conc-e_jq-p1-me1">
          4, 11, 20, 31, 44, \ldots
        </me>.
      </p>
    </statement>
    <solution permid="sec_sequences-conc-e_jq-s1">
      <p permid="sec_sequences-conc-e_jq-s1-p1">
        <m>a_n = n^2 + 4n - 1</m>.
      </p>
    </solution>
  </exercise>

  <exercise permid="sec_sequences-conc-e_mz">
    <statement>
      <p permid="sec_sequences-conc-e_mz-p1">
        Suppose the closed formula for a particular sequence is a degree 3 polynomial.
        What can you say about the closed formula for:
      </p>

      <p permid="sec_sequences-conc-e_mz-p2">
        <ol permid="sec_sequences-conc-e_mz-ol1">
          <li permid="sec_sequences-conc-e_mz-ol1-l_j">
            <p permid="sec_sequences-conc-e_mz-ol1-l_j-p1">
              The sequence of partial sums.
            </p>
          </li>

          <li permid="sec_sequences-conc-e_mz-ol1-l_s">
            <p permid="sec_sequences-conc-e_mz-ol1-l_s-p1">
              The sequence of second differences.
            </p>
          </li>
        </ol>
      </p>
    </statement>
    <solution permid="sec_sequences-conc-e_mz-s1">
      <p permid="sec_sequences-conc-e_mz-s1-p1">
        <ol permid="sec_sequences-conc-e_mz-s1-ol1">
          <li permid="sec_sequences-conc-e_mz-s1-ol1-l_j">
            <p permid="sec_sequences-conc-e_mz-s1-ol1-l_j-p1">
              The sequence of partial sums will be a degree 4 polynomial
              (its sequence of differences will be the original sequence).
            </p>
          </li>

          <li permid="sec_sequences-conc-e_mz-s1-ol1-l_s">
            <p permid="sec_sequences-conc-e_mz-s1-ol1-l_s-p1">
              The sequence of second differences will be a degree 1 polynomial - an arithmetic sequence.
            </p>
          </li>
        </ol>
      </p>
    </solution>
  </exercise>

  <exercise permid="sec_sequences-conc-e_pi">
    <statement>
      <p permid="sec_sequences-conc-e_pi-p1">
        Consider the sequence given recursively by <m>a_1 = 4</m>,
        <m>a_2 = 6</m> and <m>a_n = a_{n-1} + a_{n-2}</m>.
      </p>

      <p permid="sec_sequences-conc-e_pi-p2">
        <ol permid="sec_sequences-conc-e_pi-ol1">
          <li permid="sec_sequences-conc-e_pi-ol1-l_j">
            <p permid="sec_sequences-conc-e_pi-ol1-l_j-p1">
              Write out the first 6 terms of the sequence.
            </p>
          </li>

          <li permid="sec_sequences-conc-e_pi-ol1-l_s">
            <p permid="sec_sequences-conc-e_pi-ol1-l_s-p1">
              Could the closed formula for <m>a_n</m> be a polynomial?
              Explain.
            </p>
          </li>
        </ol>
      </p>
    </statement>
    <solution permid="sec_sequences-conc-e_pi-s1">
      <p permid="sec_sequences-conc-e_pi-s1-p1">
        <ol permid="sec_sequences-conc-e_pi-s1-ol1">
          <li permid="sec_sequences-conc-e_pi-s1-ol1-l_j"><m>4, 6, 10, 16, 26, 42, \ldots</m>.</li>

          <li permid="sec_sequences-conc-e_pi-s1-ol1-l_s">
            <p permid="sec_sequences-conc-e_pi-s1-ol1-l_s-p1">
              No, taking differences gives the original sequence back,
              so the differences will never be constant.
            </p>
          </li>
        </ol>
      </p>
    </solution>
  </exercise>

  <exercise permid="sec_sequences-conc-e_sa">
    <statement>
      <p permid="sec_sequences-conc-e_sa-p1">
        The sequence <m>-1, 0, 2, 5, 9, 14\ldots</m> has closed formula <m>a_n = \dfrac{(n+1)(n-2)}{2}</m>.
        Use this fact to find a closed formula for the sequence <m>4, 10, 18, 28, 40, \ldots</m>.
      </p>
    </statement>
    <solution permid="sec_sequences-conc-e_sa-s1">
      <p permid="sec_sequences-conc-e_sa-s1-p1">
        <m>b_n = (n+3)n</m>.
      </p>
    </solution>
  </exercise>

  <exercise permid="sec_sequences-conc-e_vj">
    <statement>
      <p permid="sec_sequences-conc-e_vj-p1">
        The in song <em>The Twelve Days of Christmas</em>,
        my true love gave to me first 1 gift,
        then 2 gifts and 1 gift, then 3 gifts, 2 gifts and 1 gift,
        and so on.
        How many gifts did my true love give me all together during the twelve days?
      </p>
    </statement>
  </exercise>

  <exercise permid="sec_sequences-conc-e_ys">
    <statement>
      <p permid="sec_sequences-conc-e_ys-p1">
        Consider the recurrence relation
        <m>a_n = 3a_{n-1} + 10 a_{n-2}</m> with first two terms <m>a_0 = 1</m> and <m>a_1 = 2</m>.
      </p>

      <p permid="sec_sequences-conc-e_ys-p2">
        <ol permid="sec_sequences-conc-e_ys-ol1">
          <li permid="sec_sequences-conc-e_ys-ol1-l_j">
            <p permid="sec_sequences-conc-e_ys-ol1-l_j-p1">
              Write out the first 5 terms of the sequence defined by this recurrence relation.
            </p>
          </li>

          <li permid="sec_sequences-conc-e_ys-ol1-l_s">
            <p permid="sec_sequences-conc-e_ys-ol1-l_s-p1">
              Solve the recurrence relation.
              That is, find a closed formula for <m>a_n</m>.
            </p>
          </li>
        </ol>
      </p>
    </statement>
    <solution permid="sec_sequences-conc-e_ys-s1">
      <p permid="sec_sequences-conc-e_ys-s1-p1">
        <ol permid="sec_sequences-conc-e_ys-s1-ol1">
          <li permid="sec_sequences-conc-e_ys-s1-ol1-l_j"><m>1, 2, 16,68, 364, \ldots</m>.</li>

          <li permid="sec_sequences-conc-e_ys-s1-ol1-l_s"><m>a_n = \frac{3}{7}(-2)^n + \frac{4}{7}5^n</m>.</li>
        </ol>
      </p>
    </solution>
  </exercise>

  <exercise permid="sec_sequences-conc-e_bk">
    <statement>
      <p permid="sec_sequences-conc-e_bk-p1">
        Consider the recurrence relation <m>a_n = 2a_{n-1} + 8a_{n-2}</m>,
        with initial terms <m>a_0 = 1</m> and <m>a_1= 3</m>.
      </p>

      <p permid="sec_sequences-conc-e_bk-p2">
        <ol permid="sec_sequences-conc-e_bk-ol1">
          <li permid="sec_sequences-conc-e_bk-ol1-l_j">
            <p permid="sec_sequences-conc-e_bk-ol1-l_j-p1">
              Find the next two terms of the sequence
              (<m>a_2</m> and <m>a_3</m>).
            </p>
          </li>

          <li permid="sec_sequences-conc-e_bk-ol1-l_s">
            <p permid="sec_sequences-conc-e_bk-ol1-l_s-p1">
              Solve the recurrence relation.
              That is, find a closed formula for the <m>n</m>th term of the sequence.
            </p>
          </li>
        </ol>
      </p>
    </statement>
    <solution permid="sec_sequences-conc-e_bk-s1">
      <p permid="sec_sequences-conc-e_bk-s1-p1">
        <ol permid="sec_sequences-conc-e_bk-s1-ol1">
          <li permid="sec_sequences-conc-e_bk-s1-ol1-l_j"><m>a_2 = 14</m>. <m>a_3 = 52</m>.</li>

          <li permid="sec_sequences-conc-e_bk-s1-ol1-l_s"><m>a_n = \frac{1}{6}(-2)^n + \frac{5}{6}4^n</m>.</li>
        </ol>
      </p>
    </solution>
  </exercise>

  <exercise permid="sec_sequences-conc-e_et">
    <statement>
      <p permid="sec_sequences-conc-e_et-p1">
        Your magic chocolate bunnies
            <idx><h>magic chocolate bunnies</h></idx>
        reproduce like rabbits:
        every large bunny produces 2 new mini bunnies each day,
        and each day every mini bunny born the previous day grows into a large bunny.
        Assume you start with 2 mini bunnies and no bunny ever dies
        (or gets eaten).
      </p>

      <p permid="sec_sequences-conc-e_et-p2">
        <ol permid="sec_sequences-conc-e_et-ol1">
          <li permid="sec_sequences-conc-e_et-ol1-l_j">
            <p permid="sec_sequences-conc-e_et-ol1-l_j-p1">
              Write out the first few terms of the sequence.
            </p>
          </li>

          <li permid="sec_sequences-conc-e_et-ol1-l_s">
            <p permid="sec_sequences-conc-e_et-ol1-l_s-p1">
              Give a recursive definition of the sequence and explain why it is correct.
            </p>
          </li>

          <li permid="sec_sequences-conc-e_et-ol1-l_b">
            <p permid="sec_sequences-conc-e_et-ol1-l_b-p1">
              Find a closed formula for the <m>n</m>th term of the sequence.
            </p>
          </li>
        </ol>
      </p>
    </statement>
    <solution permid="sec_sequences-conc-e_et-s1">
      <p permid="sec_sequences-conc-e_et-s1-p1">
        <ol permid="sec_sequences-conc-e_et-s1-ol1">
          <li permid="sec_sequences-conc-e_et-s1-ol1-l_j">
            <p permid="sec_sequences-conc-e_et-s1-ol1-l_j-p1">
              On the first day, your 2 mini bunnies become 2 large bunnies.
              On day 2, your two large bunnies produce 4 mini bunnies.
              On day 3, you have 4 mini bunnies
              (produced by your 2 large bunnies)
              plus 6 large bunnies
              (your original 2 plus the 4 newly matured bunnies).
              On day 4, you will have <m>12</m> mini bunnies (2 for each of the 6 large bunnies) plus 10 large bunnies
              (your previous 6 plus the 4 newly matured).
              The sequence of total bunnies is
              <m>2, 2, 6, 10, 22, 42\ldots</m> starting with <m>a_0 = 2</m> and <m>a_1 = 2</m>.
            </p>
          </li>

          <li permid="sec_sequences-conc-e_et-s1-ol1-l_s">
            <m>a_n = a_{n-1} + 2a_{n-2}</m>.
            This is because the number of bunnies is equal to the number of bunnies you had the previous day
            (both mini and large)
            plus 2 times the number you had the day before that
            (since all bunnies you had 2 days ago are now large and producing 2 new bunnies each).
          </li>

          <li permid="sec_sequences-conc-e_et-s1-ol1-l_b">
            <p permid="sec_sequences-conc-e_et-s1-ol1-l_b-p1">
              Using the characteristic root technique,
              we find <m>a_n = a2^n + b(-1)^n</m>,
              and we can find <m>a</m> and <m>b</m> to give <m>a_n = \frac{4}{3}2^n + \frac{2}{3}(-1)^n</m>.
            </p>
          </li>
        </ol>
      </p>
    </solution>
  </exercise>

  <exercise permid="sec_sequences-conc-e_hc">
    <statement>
      <p permid="sec_sequences-conc-e_hc-p1">
        Prove the following statements by mathematical induction:
      </p>

      <p permid="sec_sequences-conc-e_hc-p2">
        <ol permid="sec_sequences-conc-e_hc-ol1">
          <li permid="sec_sequences-conc-e_hc-ol1-l_j"><m>n! \lt n^n</m> for <m>n \ge 2</m></li>

          <li permid="sec_sequences-conc-e_hc-ol1-l_s">
            <m>\d\frac{1}{1\cdot 2} + \frac{1}{2\cdot 3} +\frac{1}{3\cdot 4}+\cdots + \frac{1}{n\cdot(n+1)} = \d\frac{n}{n+1}</m> for all <m>n \in \Z^+</m>.
          </li>

          <li permid="sec_sequences-conc-e_hc-ol1-l_b">
            <m>4^n - 1</m> is a multiple of 3 for all <m>n \in \N</m>.
          </li>

          <li permid="sec_sequences-conc-e_hc-ol1-l_k">
            <p permid="sec_sequences-conc-e_hc-ol1-l_k-p1">
              The <em>greatest</em> amount of postage you <em>cannot</em>
              make exactly using 4 and 9 cent stamps is 23 cents.
            </p>
          </li>

          <li permid="sec_sequences-conc-e_hc-ol1-l_t">
            <p permid="sec_sequences-conc-e_hc-ol1-l_t-p1">
              Every even number squared is divisible by 4.
            </p>
          </li>
        </ol>
      </p>
    </statement>
    <solution permid="sec_sequences-conc-e_hc-s1">
      <p permid="sec_sequences-conc-e_hc-s1-p1">
        <ol permid="sec_sequences-conc-e_hc-s1-ol1">
          <li permid="sec_sequences-conc-e_hc-s1-ol1-l_j">
            <p permid="sec_sequences-conc-e_hc-s1-ol1-l_j-p1">
              Hint: <m>(n+1)^{n+1} &gt; (n+1) \cdot n^{n}</m>.
            </p>
          </li>

          <li permid="sec_sequences-conc-e_hc-s1-ol1-l_s">
            <p permid="sec_sequences-conc-e_hc-s1-ol1-l_s-p1">
              Hint: This should be similar to the other sum proofs.
              The last bit comes down to adding fractions.
            </p>
          </li>

          <li permid="sec_sequences-conc-e_hc-s1-ol1-l_b">
            <p permid="sec_sequences-conc-e_hc-s1-ol1-l_b-p1">
              Hint: Write <m>4^{k+1} - 1 = 4\cdot 4^k - 4 + 3</m>.
            </p>
          </li>

          <li permid="sec_sequences-conc-e_hc-s1-ol1-l_k">
            <p permid="sec_sequences-conc-e_hc-s1-ol1-l_k-p1">
              Hint: one 9-cent stamp is 1 more than two 4-cent stamps,
              and seven 4-cent stamps is 1 more than three 9-cent stamps.
            </p>
          </li>

          <li permid="sec_sequences-conc-e_hc-s1-ol1-l_t">
            <p permid="sec_sequences-conc-e_hc-s1-ol1-l_t-p1">
              Careful to actually use induction here.
              The base case: <m>2^2 = 4</m>.
              The inductive case:
              assume <m>(2n)^2</m> is divisible by 4 and consider <m>(2n+2)^2 = (2n)^2 + 4n + 4</m>.
              This is divisible by 4 because <m>4n +4</m> clearly is,
              and by our inductive hypothesis, so is <m>(2n)^2</m>.
            </p>
          </li>
        </ol>
      </p>
    </solution>
  </exercise>

  <exercise permid="sec_sequences-conc-e_ku">
    <statement>
      <p permid="sec_sequences-conc-e_ku-p1">
        Prove <m>1^3 + 2^3 + 3^3 + \cdots + n^3 = \left(\frac{n(n+1)}{2}\right)^2</m> holds for all <m>n \ge 1</m>,
        by mathematical induction.
      </p>
    </statement>
    <solution permid="sec_sequences-conc-e_ku-s1">
      <p permid="sec_sequences-conc-e_ku-s1-p1">
        Hint: This is a straight forward induction proof.
        Note you will need to simplify
        <m>\left(\frac{n(n+1)}{2}\right)^2 + (n+1)^3</m> and get <m>\left(\frac{(n+1)(n+2)}{2}\right)^2</m>.
      </p>
    </solution>
  </exercise>

  <exercise permid="sec_sequences-conc-e_nd">
    <statement>
      <p permid="sec_sequences-conc-e_nd-p1">
        Suppose <m>a_0 = 1</m>,
        <m>a_1 = 1</m> and <m>a_n = 3a_{n-1} - 2a_{n-1}</m>.
        Prove, using strong induction,
        that <m>a_n = 1</m> for all <m>n</m>.
      </p>
    </statement>
    <solution permid="sec_sequences-conc-e_nd-s1">
      <p permid="sec_sequences-conc-e_nd-s1-p1">
        Hint: there are two base cases <m>P(0)</m> and <m>P(1)</m>.
        Then, for the inductive case,
        assume <m>P(k)</m> is true for all <m>k \lt n</m>.
        This allows you to assume <m>a_{n-1} = 1</m> and <m>a_{n-2} = 1</m>.
        Apply the recurrence relation.
      </p>
    </solution>
  </exercise>

  <exercise permid="sec_sequences-conc-e_qm">
    <statement>
      <p permid="sec_sequences-conc-e_qm-p1">
        Prove, using strong induction,
        that every positive integer can be written as the sum of distinct powers of 2.
        For example, <m>13 = 1 + 4 + 8 = 2^0 + 2^2 + 2^3</m>.
      </p>
    </statement>
    <solution permid="sec_sequences-conc-e_qm-s1">
      <p permid="sec_sequences-conc-e_qm-s1-p1">
        Note that <m>1 = 2^0</m>; this is your base case.
        Now suppose <m>k</m> can be written as the sum of distinct powers of 2 for all <m>1\le k \le n</m>.
        We can then write <m>n</m> as the sum of distinct powers of 2 as follows:
        subtract the largest power of 2 less than <m>n</m> from <m>n</m>.
        That is, write <m>n = 2^j + k</m> for the largest possible <m>j</m>.
        But <m>k</m> is now less than <m>n</m>,
        and also less than <m>2^j</m>,
        so write <m>k</m> as the sum of distinct powers of 2
        (we can do so by the inductive hypothesis).
        Thus <m>n</m> can be written as the sum of distinct powers of 2 for all <m>n \ge 1</m>.
      </p>
    </solution>
  </exercise>

  <exercise permid="sec_sequences-conc-e_te">
    <statement>
      <p permid="sec_sequences-conc-e_te-p1">
        Prove using induction that every set containing <m>n</m> elements has <m>2^n</m> different subsets for any <m>n \ge 1</m>.
      </p>
    </statement>
    <solution permid="sec_sequences-conc-e_te-s1">
      <p permid="sec_sequences-conc-e_te-s1-p1">
        Let <m>P(n)</m> be the statement,
        <q>every set containing <m>n</m> elements has <m>2^n</m> different subsets.</q>
        We will show <m>P(n)</m> is true for all <m>n \ge 1</m>.

        Base case: Any set with 1 element <m>\{a\}</m> has exactly 2 subsets:
        the empty set and the set itself.
        Thus the number of subsets is <m>2= 2^1</m>.
        Thus <m>P(1)</m> is true.

        Inductive case: Suppose <m>P(k)</m> is true for some arbitrary <m>k \ge 1</m>.
        Thus every set containing exactly <m>k</m> elements has <m>2^k</m> different subsets.
        Now consider a set containing <m>k+1</m> elements:
        <m>A = \{a_1, a_2, \ldots, a_k, a_{k+1}\}</m>.
        Any subset of <m>A</m> must either contain <m>a_{k+1}</m> or not.
        In other words, a subset of <m>A</m> is just a subset of
        <m>\{a_1, a_2,\ldots,
        a_k\}</m> with or without <m>a_{k+1}</m>.
        Thus there are <m>2^k</m> subsets of <m>A</m> which contain <m>a_{k+1}</m> and another <m>2^{k+1}</m> subsets of <m>A</m> which do not contain <m>a^{k+1}</m>.
        This gives a total of <m>2^k + 2^k = 2\cdot 2^k = 2^{k+1}</m> subsets of <m>A</m>.
        But our choice of <m>A</m> was arbitrary,
        so this works for any subset containing <m>k+1</m> elements,
        so <m>P(k+1)</m> is true.
        Therefore, by the principle of mathematical induction,
        <m>P(n)</m> is true for all <m>n \ge 1</m>.
      </p>
    </solution>
  </exercise>

</exercises>
